\documentclass[11pt,a4paper]{scrartcl}\usepackage{amssymb,bm}\usepackage{amsmath}\begin{document}
%\begin{equation}\pi(1)=\frac{length}{height }\end{equation}
\begin{align}
%\pi(1) &= \frac{length}{height }
M \ddot{z} &= (P_b - P_a)A - Mg \\
\dot{P}_b &= \frac{\gamma R T}{A z} (\dot{m}_{in} - \dot{m}_{escape} - \frac{P_b A \dot{z}}{R T})\\
\rho \frac{\partial P}{\partial x} &= \frac{\beta}{L^2}(\frac{\dot{m}_{escape}}{z})^2 + \frac{\mu}{\kappa L}(\frac{\dot{m}_{escape}}{z}) \\
\frac{\partial P}{\partial x} &= \frac{P_b - P_a}{\ell}
\end{align}

\end{document}
